theories/once.v
@@ -30,6 +30,56 @@ Proof.
     apply: IH erefl.
 Qed.
 
+Lemma is_det_tail_cut1 u p s fv t r r':
+  check_program u p ->
+  det_tree p.(sig) t ->
+  runT' u p fv s t r -> 
+  runT' u p fv s (And t [::cut] (TA cut)) r' -> 
+  match r, r' with
+  | None, None  => true
+  | Some s1, Some s2 => s1.1 = s2.1
+  | _, _ => false
+  end.
+Proof.
+  move=> H1 + [b'[c' H2]].
+  elim_run H2 H1 => dA.
+    { move=> [b[c]]; inversion 1; subst.
+      by move: H; rewrite rew_pa sA//.
+      move: H0 => /=; rewrite sA => -[???]; subst.
+      inversion H3; subst => //=.
+        by rewrite next_subst_and//=success_cut sA ges_subst_cutl//.
+        by move: H0; rewrite rew_pa success_cut sA.
+        by move: H0; rewrite rew_pa success_failed//?success_cut sA//.
+        by move: H0; rewrite/=success_cut sA.
+      by move: H; rewrite rew_pa success_failed sA//.
+      by move: H; rewrite /=sA.
+    }
+Abort.
+
+(* Proof.
+  move=> r [s'[r' H]].
+  remember (And _ _ _) as t' eqn:Ht'.
+  elim_run H l Ht'.
+  - by move: sA; rewrite rew_pa => /andP[]//.
+  - move: pA eA; rewrite rew_pa/= !push.
+    case: ifP => sl pA [???]; subst.
+    rewrite -success_cut in sl.
+    inversion rB; subst; simpl in *; eauto.
+    - rewrite sl prune_cutl//.
+    - rewrite/=; eauto.
+    - move: H0; rewrite/=sl => -[???]; subst.
+      by move: H; rewrite rew_pa sl.
+    - move: H0; rewrite sl => -[?]; subst.
+      by move: H; rewrite rew_pa success_failed//=sl.
+  - by apply: IH erefl.
+  - move: fA nA; rewrite rew_pa/=.
+    move=> /orP[fl|/andP[]]//.
+    rewrite fl failed_success//.
+    case nl: prune => //=[l'][?]; subst. 
+    apply: IH erefl.
+Qed. *)
+
+
 Section once.
 
   Variable once_sym: P.
@@ -41,10 +91,10 @@ Section once.
       premises := call (X) :: [::cut]
     |}.
 
-  Definition once_sig := arr i  (b (d Pred)) (b (d Func)).
+  Definition once_sig := arr  (b (d Pred)) (b (d Func)).
 
   Definition once_sigS : sigT :=
-    [fmap].[once_sym <- once_sig].
+    [fmap].[once_sym <- (1, once_sig)].
 
   Definition no_once (r: seq R) :=
     forall x, x \in r -> 
@@ -59,16 +109,16 @@ Section once.
       p.(rules) = once_impl :: r /\ no_once r.
 
   Lemma once_sigP sig:
-    (sig + once_sigS).[? once_sym] = Some once_sig.
+    (sig + once_sigS).[? once_sym] = Some (1, once_sig).
   Proof. by rewrite/once_sigS !FmapE.fmapE eqxx/= fsetU0 in_fset1 eqxx. Qed.
 
   Lemma get_modes_rev_once_sym t:
-    get_modes_rev (Tm_App (Tm_P once_sym) t) once_sig = [:: i].
+    get_modes_rev (Tm_App (Tm_P once_sym) t) once_sig = 1.
   Proof. by []. Qed.
 
   Lemma no_once_select u t rs s:
     no_once rs ->
-    select u (Tm_App (Tm_P once_sym) t) [:: i] rs s = (fset0, [::]).
+    select u (Tm_App (Tm_P once_sym) t) 0 1 rs s = (fset0, [::]).
   Proof.
     elim: rs t s => //= -[hd bo] xs IH t s/= H1.
     have {}IH := IH _ _ (no_once_cons H1).
@@ -96,9 +146,9 @@ Section once.
   Qed.
 
 
-  Lemma id_det_once u p s t:
+  Lemma id_det_once u p s t fv:
     prog_once p ->
-    is_det u p s (vars_tm t `|` vars_sigma s) (TA (call (Tm_App (Tm_P once_sym) t))).
+    is_det u p s fv (TA (call (Tm_App (Tm_P once_sym) t))).
   Proof.
     case: p => -[|r rs] sig []//= HS; first by move=> /(_ [::]) [].
     move=> /(_ rs) [[?] H]; subst.
@@ -107,19 +157,23 @@ Section once.
     move: H1; rewrite/=/bc [get_tm_hd _]/=.
     cbn iota.
     rewrite once_sigP/=.
+    rewrite fset0U.
     case X: fresh_rules => [fvx' rs'].
     rewrite/fresh_rule/= fset0U codomf0/= fsetU0/rename cat0f.
     rewrite/fresh_tm inE eqxx get_modes_rev_once_sym ren_app ren_V ren_P.
     rewrite in_fnd; first by rewrite inE.
-    have:= fresh_rules_sub rs (vars_tm t `|` vars_sigma s).
-    rewrite X => /= HH.
-    move=> H1/=; rewrite eqxx/= ffunE matching_V//=; last first.
-      apply/fsubset_trans.
-        apply/mut_excl.vars_deref/fsubsetUr.
-        apply/fsubsetUl.
-        by apply/fsubset_trans/fsubsetUr.
-      move: HH; rewrite fsubUset => /andP[_ Hx].
-      by apply/fsubset_trans/fsubsetUr.
+    move=> H1/=.
+    rewrite eqxx/=.
+    rewrite ffunE matching_V; last first.
+      rewrite fsubsetU//=; apply/orP; right.
+      move: X; rewrite [fresh_rules _ _]surjective_pairing => -[??]; subst.
+      apply/fsubset_trans/fresh_rules_sub.
+      by rewrite -fsetUA fsetUC -!fsetUA fsubsetUl.
+      move: X; rewrite [fresh_rules _ _]surjective_pairing => -[??]; subst.
+      rewrite fsubsetU//=; apply/orP; right.
+      apply/fsubset_trans/fresh_rules_sub.
+      by rewrite -fsetUA fsubsetUl.
+    move=>/=.
     rewrite no_once_select//=.
     rewrite/vars_sigma/= /varsU_rule/varsU_rhead/varsU_rprem/= fset0U/=.
     rewrite !fsetUA/= !fsetU0.
